Enqueue miracle?

BoundedQueue.dfy
@@ -7,20 +7,23 @@ class {:autocontracts} BoundedQueue<T(0)> {
     var last: nat
 
     predicate Valid()
+        reads this,q
     {
         0 <= n <= q.Length &&
         0 <= first < q.Length &&
         0 <= last < q.Length &&
         q.Length > 0 &&
-        (first == last) <==> (n == 0 || n == q.Length) &&
-        (n > 0 && first < last) ==> (n == last - first) &&
-        (n > 0 && first >= last) ==> (n == (q.Length + last - first))
+        ((first == last) <==> (n == 0 || n == q.Length)) &&
+        ((n > 0 && first < last) ==> (n == last - first)) &&
+        ((n > 0 && first >= last) ==> (n == (q.Length + last - first)))
+         //&&
+        //(n == 0 && first == last) ==> (n == (last - first) || n == first - last)
  
     }
 
     constructor (length : nat)
         requires length > 0
-        ensures q.Length > 0
+        ensures Valid()
         //ensures contents == []
     {
         q := new T[length];
@@ -31,14 +34,20 @@ class {:autocontracts} BoundedQueue<T(0)> {
     }
 
     function method IsEmpty(): bool
+        //reads this,q
+        requires Valid()
+        ensures Valid()
         //ensures IsEmpty() <==> contents == []
-        ensures IsEmpty() ==> first == last
+        //ensures IsEmpty() ==> first == last
     {
         n == 0
     }
 
     
     function method IsFull(): bool
+        //reads this,q
+        requires Valid()
+        ensures Valid()
         ensures IsFull() <==> n == q.Length
         //ensures !IsFull() ==> last > 0
     {
@@ -47,32 +56,93 @@ class {:autocontracts} BoundedQueue<T(0)> {
 
     // Adds the item to this queue 
     method Enqueue(item: T)
+        modifies this,q
+        requires Valid()
+        ensures Valid()
         requires !IsFull()
+        ensures q == old(q)
+        /*ensures n < q.Length ==> !IsFull()
+        ensures n == q.Length ==> IsFull()*/
     {  
+        q[last] := item;
         assert n != q.Length;
+        if (first > last){            
+            last := last + 1;
+            n := n + 1;
+            assert Valid();
+        } else if (first < last) { //first >= last
+            if (last + 1 == q.Length){
+                last := 0;
+                n := n + 1;
+            } else {
+                last := last + 1;
+                n := n + 1;
+            }
+        } else if (IsEmpty()){ //first == last
+                assert n == 0;
+                assert first == last;
+                //n := n + 1;
+            if (last + 1 == q.Length && first + 1 == q.Length) {
+                last := 0;
+                n := n + 1;
+                assert n != 0;
+               //assert last < first;
+                //assert n != q.Length;
+                
+                //n := q.Length + last - first    
+            } else {
+                last := last + 1;
+                n := n + 1;
+            }
+        }
     }
 
     // Removes and returns the item on this queue that was least recently added 
     method Dequeue() returns (item: T)
+        requires Valid()
+        ensures Valid()
         requires !IsEmpty()
     {
         assert n > 0;
-        if (first < last){
-            assert n == last - first;
-            first := first + 1;
-            n := n - 1;
-        } else {
-            assert n > 0 && first >= last;
-            assert n == (q.Length + last - first);
-        }
+        
     }
 
     // Returns the item least recently added to this queue 
     function method Peek(): T
+        //reads this,q
+        requires Valid()
+        ensures Valid()
         requires !IsEmpty()
         //ensures contents == old(contents)
     {   
+        assert  0 <= first ;
         q[first]
     }
 
+    function method Size(): nat
+        //reads this,q
+        requires Valid()
+        ensures Valid()
+        //ensures contents == old(contents)
+    {   
+        n
+    }
+
+}
+
+method Main() {
+  print "BoundedQueue\n";    
+  var q := new BoundedQueue<int>(3);
+  //---------------------
+  print q.Size(); print "\n";
+  if (!q.IsFull()){
+    q.Enqueue(-1);
+  }
+  if (!q.IsFull()){
+    q.Enqueue(-2);
+  } 
+  print q.Size(); print "\n";
+  if(!q.IsEmpty()){
+      print q.Peek(); print "\n";
+  }
 }
